Pes simulation
Establish the relationship between pes simulation and ifs refinement

PiCore_Sim.thy
@@ -18,29 +18,16 @@ definition rel_guard_and :: "'s\<^sub>c set \<Rightarrow> 's\<^sub>a set \<Right
   where "rel_guard_and g\<^sub>c g\<^sub>a = {(\<sigma>, \<Sigma>). \<sigma> \<in> g\<^sub>c \<and> \<Sigma> \<in> g\<^sub>a}"
 
 locale PiCore_Sim =
-  InfoFlow\<^sub>c: InfoFlow ptran\<^sub>c petran\<^sub>c fin_com\<^sub>c C0\<^sub>c step\<^sub>c interference\<^sub>c vpeq\<^sub>c obs\<^sub>c dome\<^sub>c +
-  InfoFlow\<^sub>a: InfoFlow ptran\<^sub>a petran\<^sub>a fin_com\<^sub>a C0\<^sub>a step\<^sub>a interference\<^sub>a vpeq\<^sub>a obs\<^sub>a dome\<^sub>a
+  Event\<^sub>c: event ptran\<^sub>c petran\<^sub>c fin_com\<^sub>c +
+  Event\<^sub>a: event ptran\<^sub>a petran\<^sub>a fin_com\<^sub>a
   for ptran\<^sub>c :: "'Env\<^sub>c \<Rightarrow> (('prog\<^sub>c \<times> 's\<^sub>c) \<times> 'prog\<^sub>c \<times> 's\<^sub>c) set" 
   and petran\<^sub>c :: "'Env\<^sub>c \<Rightarrow> 'prog\<^sub>c \<times> 's\<^sub>c \<Rightarrow> 'prog\<^sub>c \<times> 's\<^sub>c \<Rightarrow> bool" 
   and fin_com\<^sub>c :: "'prog\<^sub>c"
-  and C0\<^sub>c  :: "('l\<^sub>c,'k\<^sub>c,'s\<^sub>c,'prog\<^sub>c) pesconf"
-  and step\<^sub>c :: "('l\<^sub>c,'k\<^sub>c,'s\<^sub>c,'prog\<^sub>c, 'd) action \<Rightarrow> (('l\<^sub>c,'k\<^sub>c,'s\<^sub>c,'prog\<^sub>c) pesconf \<times> ('l\<^sub>c,'k\<^sub>c,'s\<^sub>c,'prog\<^sub>c) pesconf) set"
-  and interference\<^sub>c :: "'d \<Rightarrow> 'd \<Rightarrow> bool" 
-  and vpeq\<^sub>c :: "'s\<^sub>c \<Rightarrow> 'd \<Rightarrow> 's\<^sub>c \<Rightarrow> bool" ("(_ \<sim>\<^sub>c_\<sim>\<^sub>c _)" [70,69,70] 60)
-  and obs\<^sub>c :: "'s\<^sub>c \<Rightarrow> 'd \<Rightarrow> 'o\<^sub>c" 
-  and dome\<^sub>c :: "'s\<^sub>c \<Rightarrow> ('l\<^sub>c, 'k\<^sub>c, 's\<^sub>c, 'prog\<^sub>c) event \<Rightarrow> 'd"
   and ptran\<^sub>a :: "'Env\<^sub>a \<Rightarrow> (('prog\<^sub>a \<times> 's\<^sub>a) \<times> 'prog\<^sub>a \<times> 's\<^sub>a) set"
   and petran\<^sub>a :: "'Env\<^sub>a \<Rightarrow> 'prog\<^sub>a \<times> 's\<^sub>a \<Rightarrow> 'prog\<^sub>a \<times> 's\<^sub>a \<Rightarrow> bool" 
-  and fin_com\<^sub>a :: "'prog\<^sub>a"
-  and C0\<^sub>a :: "('l\<^sub>a, 'k\<^sub>a, 's\<^sub>a, 'prog\<^sub>a) pesconf"
-  and step\<^sub>a :: "('l\<^sub>a,'k\<^sub>a,'s\<^sub>a,'prog\<^sub>a, 'd) action \<Rightarrow> (('l\<^sub>a,'k\<^sub>a,'s\<^sub>a,'prog\<^sub>a) pesconf \<times> ('l\<^sub>a,'k\<^sub>a,'s\<^sub>a,'prog\<^sub>a) pesconf) set" 
-  and interference\<^sub>a :: "'d \<Rightarrow> 'd \<Rightarrow> bool" 
-  and vpeq\<^sub>a ::  "'s\<^sub>a \<Rightarrow> 'd \<Rightarrow> 's\<^sub>a \<Rightarrow> bool" ("(_ \<sim>\<^sub>a_\<sim>\<^sub>a _)" [70,69,70] 60)
-  and obs\<^sub>a :: "'s\<^sub>a \<Rightarrow> 'd \<Rightarrow> 'o\<^sub>a" 
-  and dome\<^sub>a :: "'s\<^sub>a \<Rightarrow> ('l\<^sub>a, 'k\<^sub>a, 's\<^sub>a, 'prog\<^sub>a) event \<Rightarrow> 'd" +
-fixes 
-      sim_e :: "('l\<^sub>c, 'k\<^sub>c, 's\<^sub>c, 'prog\<^sub>c) event \<Rightarrow> ('l\<^sub>a, 'k\<^sub>a, 's\<^sub>a, 'prog\<^sub>a) event option"
-  and prog_sim :: "['Env\<^sub>c, ('s\<^sub>c,'prog\<^sub>c) pconf, ('s\<^sub>c \<times> 's\<^sub>c) set, ('s\<^sub>c \<times> 's\<^sub>c) set, 
+  and fin_com\<^sub>a :: "'prog\<^sub>a" +
+fixes
+      prog_sim :: "['Env\<^sub>c, ('s\<^sub>c,'prog\<^sub>c) pconf, ('s\<^sub>c \<times> 's\<^sub>c) set, ('s\<^sub>c \<times> 's\<^sub>c) set, 
                   ('s\<^sub>c \<times> 's\<^sub>a) set, 'prog\<^sub>c \<Rightarrow> 'prog\<^sub>a option, ('s\<^sub>c \<times> 's\<^sub>a) set,
                   'Env\<^sub>a, ('s\<^sub>a,'prog\<^sub>a) pconf, ('s\<^sub>a \<times> 's\<^sub>a) set, ('s\<^sub>a \<times> 's\<^sub>a) set] \<Rightarrow> bool" 
   ("'(_,_,_,_')/ \<preceq>\<^sub>p \<^sub>'(\<^sub>_\<^sub>;\<^sub>_\<^sub>;\<^sub>_\<^sub>') /'(_,_,_,_')" [81,81,81,81,81,81,81,81,81,81,81] 100)
@@ -49,9 +36,6 @@ fixes
                   'Env\<^sub>a, 'prog\<^sub>a, ('s\<^sub>a \<times> 's\<^sub>a) set, ('s\<^sub>a \<times> 's\<^sub>a) set] \<Rightarrow> bool" 
   ("'(_,_,_,_')/ \<preceq>\<^sub>p \<^sub>'(\<^sub>_\<^sub>;\<^sub>_\<^sub>;\<^sub>_\<^sub>\<rhd>\<^sub>_\<^sub>')  /'(_,_,_,_')" [81,81,81,81,81,81,81,81,81,81,81,81] 100)
 assumes
-  all_evts_are_basic: "(\<forall>e \<in> all_evts (getspc C0\<^sub>c). is_basicevt e) \<and> 
-                       (\<forall>e \<in> all_evts (getspc C0\<^sub>a). is_basicevt e)" and
-  intefere_same : "interference\<^sub>c  = interference\<^sub>a" and 
   prog_sim_validity: "(\<Gamma>\<^sub>c, (P\<^sub>c, s\<^sub>c), R\<^sub>c, G\<^sub>c) \<preceq>\<^sub>p \<^sub>(\<^sub>\<alpha>\<^sub>;\<^sub>\<zeta>\<^sub>;\<^sub>\<gamma>\<^sub>) (\<Gamma>\<^sub>a, (P\<^sub>a, s\<^sub>a), R\<^sub>a, G\<^sub>a) \<Longrightarrow>
                             (s\<^sub>c, s\<^sub>a) \<in> \<alpha> \<and>
 
@@ -71,47 +55,48 @@ assumes
                            (\<Gamma>\<^sub>c, (P\<^sub>c, s\<^sub>c), R\<^sub>c, G\<^sub>c) \<preceq>\<^sub>p \<^sub>(\<^sub>\<alpha>\<^sub>;\<^sub>\<zeta>\<^sub>;\<^sub>\<gamma>\<^sub>) (\<Gamma>\<^sub>a, (P\<^sub>a, s\<^sub>a), R\<^sub>a, G\<^sub>a)"
 begin
 
+
 lemma prog_sim_pre_implies_inv : "(\<Gamma>\<^sub>c,P\<^sub>c,R\<^sub>c,G\<^sub>c) \<preceq>\<^sub>p \<^sub>(\<^sub>\<alpha>\<^sub>;\<^sub>\<zeta>\<^sub>;\<^sub>\<xi>\<^sub>\<rhd>\<^sub>\<gamma>\<^sub>)  (\<Gamma>\<^sub>a,P\<^sub>a,R\<^sub>a,G\<^sub>a) \<Longrightarrow> \<xi> \<subseteq> \<alpha>"
   by (meson prog_sim_pre_validity prog_sim_validity subrelI)
 
 abbreviation ptran\<^sub>c' :: "'Env\<^sub>c \<Rightarrow> ('s\<^sub>c,'prog\<^sub>c) pconf \<Rightarrow> ('s\<^sub>c,'prog\<^sub>c) pconf \<Rightarrow> bool" ("_ \<turnstile>\<^sub>c _ -c\<rightarrow> _" [81,81] 80)
-  where "ptran\<^sub>c' \<equiv> InfoFlow\<^sub>c.ptran'"
+  where "ptran\<^sub>c' \<equiv> Event\<^sub>c.ptran'"
 
 abbreviation ptrans\<^sub>c :: "'Env\<^sub>c \<Rightarrow> ('s\<^sub>c,'prog\<^sub>c) pconf \<Rightarrow> ('s\<^sub>c,'prog\<^sub>c) pconf \<Rightarrow> bool" ("_ \<turnstile>\<^sub>c _ c*\<rightarrow> _" [81,81] 80)
-  where "ptrans\<^sub>c \<equiv> InfoFlow\<^sub>c.ptrans"
+  where "ptrans\<^sub>c \<equiv>  Event\<^sub>c.ptrans"
 
 abbreviation etran\<^sub>c ::  "'Env\<^sub>c \<Rightarrow> ('l\<^sub>c,'k,'s\<^sub>c,'prog\<^sub>c) econf \<Rightarrow> ('l\<^sub>c,'k,'s\<^sub>c,'prog\<^sub>c) actk \<Rightarrow> 
                         ('l\<^sub>c,'k,'s\<^sub>c,'prog\<^sub>c) econf \<Rightarrow> bool" ("_ \<turnstile>\<^sub>c _ -et-_\<rightarrow> _" [81,81,81] 80)
-  where "etran\<^sub>c \<equiv> InfoFlow\<^sub>c.etran"
+  where "etran\<^sub>c \<equiv>  Event\<^sub>c.etran"
 
 
 abbreviation estran\<^sub>c :: "'Env\<^sub>c \<Rightarrow> ('l\<^sub>c,'k,'s\<^sub>c,'prog\<^sub>c) esconf \<Rightarrow> ('l\<^sub>c,'k,'s\<^sub>c,'prog\<^sub>c) actk \<Rightarrow> 
                         ('l\<^sub>c,'k,'s\<^sub>c,'prog\<^sub>c) esconf \<Rightarrow> bool" ("_ \<turnstile>\<^sub>c _ -es-_\<rightarrow> _" [81,81] 80)
-  where "estran\<^sub>c \<equiv> InfoFlow\<^sub>c.estran"
+  where "estran\<^sub>c \<equiv>  Event\<^sub>c.estran"
 
 abbreviation pestran\<^sub>c :: "'Env\<^sub>c \<Rightarrow> ('l\<^sub>c,'k,'s\<^sub>c,'prog\<^sub>c) pesconf \<Rightarrow> ('l\<^sub>c,'k,'s\<^sub>c,'prog\<^sub>c) actk \<Rightarrow> 
                         ('l\<^sub>c,'k,'s\<^sub>c,'prog\<^sub>c) pesconf \<Rightarrow> bool" ("_ \<turnstile>\<^sub>c _ -pes-_\<rightarrow> _" [70,70] 60)
-  where "pestran\<^sub>c \<equiv> InfoFlow\<^sub>c.pestran"
+  where "pestran\<^sub>c \<equiv>  Event\<^sub>c.pestran"
 
 
 abbreviation ptran\<^sub>a' :: "'Env\<^sub>a \<Rightarrow> ('s\<^sub>a,'prog\<^sub>a) pconf \<Rightarrow> ('s\<^sub>a,'prog\<^sub>a) pconf \<Rightarrow> bool" ("_ \<turnstile>\<^sub>a _ -c\<rightarrow> _" [81,81] 80)
-  where "ptran\<^sub>a' \<equiv> InfoFlow\<^sub>a.ptran'"
+  where "ptran\<^sub>a' \<equiv>  Event\<^sub>a.ptran'"
 
 abbreviation ptrans\<^sub>a :: "'Env\<^sub>a \<Rightarrow> ('s\<^sub>a,'prog\<^sub>a) pconf \<Rightarrow> ('s\<^sub>a,'prog\<^sub>a) pconf \<Rightarrow> bool" ("_ \<turnstile>\<^sub>a _ c*\<rightarrow> _" [81,81] 80)
-  where "ptrans\<^sub>a \<equiv> InfoFlow\<^sub>a.ptrans"
+  where "ptrans\<^sub>a \<equiv> Event\<^sub>a.ptrans"
 
 abbreviation etran\<^sub>a ::  "'Env\<^sub>a \<Rightarrow> ('l\<^sub>a,'k,'s\<^sub>a,'prog\<^sub>a) econf \<Rightarrow> ('l\<^sub>a,'k,'s\<^sub>a,'prog\<^sub>a) actk \<Rightarrow> 
                         ('l\<^sub>a,'k,'s\<^sub>a,'prog\<^sub>a) econf \<Rightarrow> bool" ("_ \<turnstile>\<^sub>a _ -et-_\<rightarrow> _" [81,81,81] 80)
-  where "etran\<^sub>a \<equiv> InfoFlow\<^sub>a.etran"
+  where "etran\<^sub>a \<equiv> Event\<^sub>a.etran"
 
 
 abbreviation estran\<^sub>a :: "'Env\<^sub>a \<Rightarrow> ('l\<^sub>a,'k,'s\<^sub>a,'prog\<^sub>a) esconf \<Rightarrow> ('l\<^sub>a,'k,'s\<^sub>a,'prog\<^sub>a) actk \<Rightarrow> 
                         ('l\<^sub>a,'k,'s\<^sub>a,'prog\<^sub>a) esconf \<Rightarrow> bool" ("_ \<turnstile>\<^sub>a _ -es-_\<rightarrow> _" [81,81] 80)
-  where "estran\<^sub>a \<equiv> InfoFlow\<^sub>a.estran"
+  where "estran\<^sub>a \<equiv> Event\<^sub>a.estran"
 
 abbreviation pestran\<^sub>a :: "'Env\<^sub>a \<Rightarrow> ('l\<^sub>a,'k,'s\<^sub>a,'prog\<^sub>a) pesconf \<Rightarrow> ('l\<^sub>a,'k,'s\<^sub>a,'prog\<^sub>a) actk \<Rightarrow> 
                         ('l\<^sub>a,'k,'s\<^sub>a,'prog\<^sub>a) pesconf \<Rightarrow> bool" ("_ \<turnstile>\<^sub>a _ -pes-_\<rightarrow> _" [70,70] 60)
-  where "pestran\<^sub>a \<equiv> InfoFlow\<^sub>a.pestran"
+  where "pestran\<^sub>a \<equiv> Event\<^sub>a.pestran"
 
 coinductive e_sim :: "['Env\<^sub>c, ('l\<^sub>c,'k,'s\<^sub>c,'prog\<^sub>c) econf, ('s\<^sub>c \<times> 's\<^sub>c) set, ('s\<^sub>c \<times> 's\<^sub>c) set, 
                   ('s\<^sub>c \<times> 's\<^sub>a) set, 'prog\<^sub>c \<Rightarrow> 'prog\<^sub>a option, ('s\<^sub>c \<times> 's\<^sub>a) set,
@@ -121,18 +106,18 @@ coinductive e_sim :: "['Env\<^sub>c, ('l\<^sub>c,'k,'s\<^sub>c,'prog\<^sub>c) ec
                   
                   (\<forall>ec e\<^sub>c' x\<^sub>c' k. (\<Gamma>\<^sub>c \<turnstile>\<^sub>c (e\<^sub>c, s\<^sub>c, x\<^sub>c) -et-((EvtEnt ec)\<sharp>k)\<rightarrow> (e\<^sub>c', s\<^sub>c, x\<^sub>c')) \<longrightarrow> (\<exists>ea e\<^sub>a' x\<^sub>a'.
                    (\<Gamma>\<^sub>a \<turnstile>\<^sub>a (e\<^sub>a, s\<^sub>a, x\<^sub>a) -et-((EvtEnt ea)\<sharp>k)\<rightarrow> (e\<^sub>a', s\<^sub>a, x\<^sub>a')) \<and>
-                   (\<Gamma>\<^sub>c, (e\<^sub>c', s\<^sub>c, x\<^sub>c'), R\<^sub>c, G\<^sub>c) \<preceq>\<^sub>e \<^sub>(\<^sub>\<alpha>\<^sub>;\<^sub>\<zeta>\<^sub>;\<^sub>\<gamma>\<^sub>) (\<Gamma>\<^sub>a, (e\<^sub>a', s\<^sub>a, x\<^sub>a'), R\<^sub>a, G\<^sub>a))) \<and>
+                   (\<Gamma>\<^sub>c, (e\<^sub>c', s\<^sub>c, x\<^sub>c'), R\<^sub>c, G\<^sub>c) \<preceq>\<^sub>e \<^sub>(\<^sub>\<alpha>\<^sub>;\<^sub>\<zeta>\<^sub>;\<^sub>\<gamma>\<^sub>) (\<Gamma>\<^sub>a, (e\<^sub>a', s\<^sub>a, x\<^sub>a'), R\<^sub>a, G\<^sub>a))) ;
 
                    (\<forall>Pc e\<^sub>c' s\<^sub>c' k. (\<Gamma>\<^sub>c \<turnstile>\<^sub>c (e\<^sub>c, s\<^sub>c, x\<^sub>c) -et-((Cmd Pc)\<sharp>k)\<rightarrow> (e\<^sub>c', s\<^sub>c', x\<^sub>c)) \<and> \<zeta> Pc = None \<longrightarrow> 
-                   (s\<^sub>c, s\<^sub>c') \<in> G\<^sub>c \<and> (\<Gamma>\<^sub>c, (e\<^sub>c', s\<^sub>c', x\<^sub>c), R\<^sub>c, G\<^sub>c) \<preceq>\<^sub>e \<^sub>(\<^sub>\<alpha>\<^sub>;\<^sub>\<zeta>\<^sub>;\<^sub>\<gamma>\<^sub>) (\<Gamma>\<^sub>a, (e\<^sub>a, s\<^sub>a, x\<^sub>a), R\<^sub>a, G\<^sub>a)) \<and>
+                   (s\<^sub>c, s\<^sub>c') \<in> G\<^sub>c \<and> (\<Gamma>\<^sub>c, (e\<^sub>c', s\<^sub>c', x\<^sub>c), R\<^sub>c, G\<^sub>c) \<preceq>\<^sub>e \<^sub>(\<^sub>\<alpha>\<^sub>;\<^sub>\<zeta>\<^sub>;\<^sub>\<gamma>\<^sub>) (\<Gamma>\<^sub>a, (e\<^sub>a, s\<^sub>a, x\<^sub>a), R\<^sub>a, G\<^sub>a)) ;
 
                   (\<forall>Pc e\<^sub>c' s\<^sub>c' k Pa. (\<Gamma>\<^sub>c \<turnstile>\<^sub>c (e\<^sub>c, s\<^sub>c, x\<^sub>c) -et-((Cmd Pc)\<sharp>k)\<rightarrow> (e\<^sub>c', s\<^sub>c', x\<^sub>c)) \<and> \<zeta> Pc = Some Pa \<longrightarrow> 
                    (\<exists>e\<^sub>a' s\<^sub>a'. 
                    (\<Gamma>\<^sub>a \<turnstile>\<^sub>a (e\<^sub>a, s\<^sub>a, x\<^sub>a) -et-((Cmd Pa)\<sharp>k)\<rightarrow> (e\<^sub>a', s\<^sub>a', x\<^sub>a)) \<and> (s\<^sub>c, s\<^sub>c') \<in> G\<^sub>c \<and> (s\<^sub>a, s\<^sub>a') \<in> G\<^sub>a \<and> 
-                   (\<Gamma>\<^sub>c, (e\<^sub>c', s\<^sub>c', x\<^sub>c), R\<^sub>c, G\<^sub>c) \<preceq>\<^sub>e \<^sub>(\<^sub>\<alpha>\<^sub>;\<^sub>\<zeta>\<^sub>;\<^sub>\<gamma>\<^sub>) (\<Gamma>\<^sub>a, (e\<^sub>a', s\<^sub>a', x\<^sub>a), R\<^sub>a, G\<^sub>a))) \<and>
+                   (\<Gamma>\<^sub>c, (e\<^sub>c', s\<^sub>c', x\<^sub>c), R\<^sub>c, G\<^sub>c) \<preceq>\<^sub>e \<^sub>(\<^sub>\<alpha>\<^sub>;\<^sub>\<zeta>\<^sub>;\<^sub>\<gamma>\<^sub>) (\<Gamma>\<^sub>a, (e\<^sub>a', s\<^sub>a', x\<^sub>a), R\<^sub>a, G\<^sub>a))) ;
 
 
-                   (e\<^sub>c = AnonyEvent fin_com\<^sub>c \<longrightarrow> e\<^sub>a = AnonyEvent fin_com\<^sub>a \<and> (s\<^sub>c, s\<^sub>a) \<in> \<gamma> \<and> \<gamma> \<subseteq> \<alpha>) \<and> 
+                   (e\<^sub>c = AnonyEvent fin_com\<^sub>c \<longrightarrow> e\<^sub>a = AnonyEvent fin_com\<^sub>a \<and> (s\<^sub>c, s\<^sub>a) \<in> \<gamma> \<and> \<gamma> \<subseteq> \<alpha>) ; 
 
                    (\<forall>s\<^sub>c' s\<^sub>a'. ((s\<^sub>c, s\<^sub>c'), (s\<^sub>a, s\<^sub>a')) \<in> ((R\<^sub>c, R\<^sub>a \<union> Id)\<^sub>\<alpha>) \<longrightarrow> 
                      (\<Gamma>\<^sub>c, (e\<^sub>c, s\<^sub>c', x\<^sub>c'), R\<^sub>c, G\<^sub>c) \<preceq>\<^sub>e \<^sub>(\<^sub>\<alpha>\<^sub>;\<^sub>\<zeta>\<^sub>;\<^sub>\<gamma>\<^sub>) (\<Gamma>\<^sub>a, (e\<^sub>a, s\<^sub>a', x\<^sub>a'), R\<^sub>a, G\<^sub>a))      
@@ -159,11 +144,11 @@ proof-
      and a1: "\<Gamma>\<^sub>c \<turnstile>\<^sub>c (AnonyEvent P\<^sub>c, s\<^sub>c, x\<^sub>c) -et-Cmd Pc\<sharp>k\<rightarrow> (e\<^sub>c', s\<^sub>c', x\<^sub>c)"
      and a2: "\<zeta> Pc = None"
   from a1 have "(Pc = P\<^sub>c) \<and> (\<exists>P\<^sub>c'. \<Gamma>\<^sub>c \<turnstile>\<^sub>c (P\<^sub>c, s\<^sub>c) -c\<rightarrow> (P\<^sub>c', s\<^sub>c') \<and> e\<^sub>c' = AnonyEvent P\<^sub>c')"
-    apply (rule InfoFlow\<^sub>c.etran.cases, simp_all)
+    apply (rule Event\<^sub>c.etran.cases, simp_all)
     by (metis act.inject(1) actk.ext_inject get_actk_def)
   then obtain P\<^sub>c' where a3: "Pc = P\<^sub>c \<and> \<Gamma>\<^sub>c \<turnstile>\<^sub>c (P\<^sub>c, s\<^sub>c) -c\<rightarrow> (P\<^sub>c', s\<^sub>c') \<and> e\<^sub>c' = AnonyEvent P\<^sub>c'" by auto
   with a0 a2 have "(s\<^sub>c, s\<^sub>c') \<in> G\<^sub>c \<and> (\<Gamma>\<^sub>c, (P\<^sub>c', s\<^sub>c'), R\<^sub>c, G\<^sub>c) \<preceq>\<^sub>p \<^sub>(\<^sub>\<alpha>\<^sub>;\<^sub>\<zeta>\<^sub>;\<^sub>\<gamma>\<^sub>) (\<Gamma>\<^sub>a, (P\<^sub>a, s\<^sub>a), R\<^sub>a, G\<^sub>a)"
-    by (meson InfoFlow\<^sub>c.ptran'_def prog_sim_validity)
+    by (meson Event\<^sub>c.ptran'_def prog_sim_validity)
   then show ?thesis
     by (simp add: a3)
 qed
@@ -178,15 +163,15 @@ proof-
      and a1: "\<Gamma>\<^sub>c \<turnstile>\<^sub>c (AnonyEvent P\<^sub>c, s\<^sub>c, x\<^sub>c) -et-Cmd Pc\<sharp>k\<rightarrow> (e\<^sub>c', s\<^sub>c', x\<^sub>c)"
      and a2: "\<zeta> Pc = Some Pa"  
   from a1 have "Pc = P\<^sub>c \<and> (\<exists>P\<^sub>c'. \<Gamma>\<^sub>c \<turnstile>\<^sub>c (P\<^sub>c, s\<^sub>c) -c\<rightarrow> (P\<^sub>c', s\<^sub>c') \<and> e\<^sub>c' = AnonyEvent P\<^sub>c')"
-    apply (rule InfoFlow\<^sub>c.etran.cases, simp_all)
+    apply (rule Event\<^sub>c.etran.cases, simp_all)
     by (metis act.inject(1) actk.ext_inject get_actk_def)
   then obtain P\<^sub>c' where a3: "Pc = P\<^sub>c \<and> \<Gamma>\<^sub>c \<turnstile>\<^sub>c (P\<^sub>c, s\<^sub>c) -c\<rightarrow> (P\<^sub>c', s\<^sub>c') \<and> e\<^sub>c' = AnonyEvent P\<^sub>c'" by auto
   with a0 have "\<zeta> P\<^sub>c = Some P\<^sub>a \<and> (\<exists>P\<^sub>a' s\<^sub>a'. \<Gamma>\<^sub>a \<turnstile>\<^sub>a (P\<^sub>a, s\<^sub>a) -c\<rightarrow> (P\<^sub>a', s\<^sub>a')
   \<and> (s\<^sub>c, s\<^sub>c') \<in> G\<^sub>c \<and> (s\<^sub>a, s\<^sub>a') \<in> G\<^sub>a \<and> (\<Gamma>\<^sub>c, (P\<^sub>c', s\<^sub>c'), R\<^sub>c, G\<^sub>c) \<preceq>\<^sub>p \<^sub>(\<^sub>\<alpha>\<^sub>;\<^sub>\<zeta>\<^sub>;\<^sub>\<gamma>\<^sub>) (\<Gamma>\<^sub>a, (P\<^sub>a', s\<^sub>a'), R\<^sub>a, G\<^sub>a))"
-    by (smt (verit, best) InfoFlow\<^sub>a.ptran'_def InfoFlow\<^sub>c.ptran'_def a2 option.distinct(1) prog_sim_validity)
+    by (smt (verit, best) Event\<^sub>a.ptran'_def Event\<^sub>c.ptran'_def a2 option.distinct(1) prog_sim_validity)
   then obtain P\<^sub>a' s\<^sub>a' where a4: "\<zeta> P\<^sub>c = Some P\<^sub>a \<and> \<Gamma>\<^sub>a \<turnstile>\<^sub>a (P\<^sub>a, s\<^sub>a) -c\<rightarrow> (P\<^sub>a', s\<^sub>a')\<and> (s\<^sub>c, s\<^sub>c') \<in> G\<^sub>c 
   \<and> (s\<^sub>a, s\<^sub>a') \<in> G\<^sub>a \<and> (\<Gamma>\<^sub>c, (P\<^sub>c', s\<^sub>c'), R\<^sub>c, G\<^sub>c) \<preceq>\<^sub>p \<^sub>(\<^sub>\<alpha>\<^sub>;\<^sub>\<zeta>\<^sub>;\<^sub>\<gamma>\<^sub>) (\<Gamma>\<^sub>a, (P\<^sub>a', s\<^sub>a'), R\<^sub>a, G\<^sub>a)" by auto
-  with a2 a3 show ?thesis by (metis InfoFlow\<^sub>a.AnonyEvent option.inject)
+  with a2 a3 show ?thesis by (metis Event\<^sub>a.AnonyEvent option.inject)
 qed
 
 lemma AnonyEvt_Sound_lemma : "(\<Gamma>\<^sub>c, (P\<^sub>c, s\<^sub>c), R\<^sub>c, G\<^sub>c) \<preceq>\<^sub>p \<^sub>(\<^sub>\<alpha>\<^sub>;\<^sub>\<zeta>\<^sub>;\<^sub>\<gamma>\<^sub>) (\<Gamma>\<^sub>a, (P\<^sub>a, s\<^sub>a), R\<^sub>a, G\<^sub>a)  \<Longrightarrow>
@@ -195,7 +180,7 @@ lemma AnonyEvt_Sound_lemma : "(\<Gamma>\<^sub>c, (P\<^sub>c, s\<^sub>c), R\<^sub
   apply (rule conjI)
   using prog_sim_validity apply blast
   apply (rule conjI)
-   apply (metis InfoFlow\<^sub>c.EvtSeq1 InfoFlow\<^sub>c.EvtSeq2 InfoFlow\<^sub>c.ent_spec1 InfoFlow\<^sub>c.evtent_is_basicevt event.distinct(1))
+   apply (metis Event\<^sub>c.EvtSeq1 Event\<^sub>c.EvtSeq2 Event\<^sub>c.ent_spec1 Event\<^sub>c.evtent_is_basicevt event.distinct(1))
   apply (rule conjI, clarsimp)
   apply (simp add: AnonyEvt_Sound_help1)
   apply (rule conjI, clarsimp)
@@ -203,9 +188,6 @@ lemma AnonyEvt_Sound_lemma : "(\<Gamma>\<^sub>c, (P\<^sub>c, s\<^sub>c), R\<^sub
   apply (rule conjI)
   using prog_sim_validity apply blast
   using prog_sim_validity by blast
-
-
-thm prog_sim_pre_validity
 
 theorem AnonyEvent_Sound : "(\<Gamma>\<^sub>c, P\<^sub>c, R\<^sub>c, G\<^sub>c) \<preceq>\<^sub>p \<^sub>(\<^sub>\<alpha>\<^sub>;\<^sub>\<zeta>\<^sub>;\<^sub>\<xi>\<^sub>\<rhd>\<^sub>\<gamma>\<^sub>)  (\<Gamma>\<^sub>a, P\<^sub>a, R\<^sub>a, G\<^sub>a) \<Longrightarrow>  
                             (\<Gamma>\<^sub>c, AnonyEvent P\<^sub>c, R\<^sub>c, G\<^sub>c) \<preceq>\<^sub>e \<^sub>(\<^sub>\<alpha>\<^sub>;\<^sub>\<zeta>\<^sub>;\<^sub>\<xi>\<^sub>\<rhd>\<^sub>\<gamma>\<^sub>)  (\<Gamma>\<^sub>a, AnonyEvent P\<^sub>a, R\<^sub>a, G\<^sub>a)"
@@ -223,13 +205,13 @@ proof-
      and a4: "\<Gamma>\<^sub>c \<turnstile>\<^sub>c (BasicEvent (l\<^sub>c, g\<^sub>c, P\<^sub>c), s\<^sub>c, x\<^sub>c) -et-EvtEnt ec\<sharp>k\<rightarrow> (e\<^sub>c', s\<^sub>c, x\<^sub>c')"
      and a5: "P\<^sub>a \<noteq> fin_com\<^sub>a"
   from a4 have a6: "s\<^sub>c \<in> g\<^sub>c \<and> e\<^sub>c' = AnonyEvent P\<^sub>c " 
-    apply (rule InfoFlow\<^sub>c.etran.cases, simp_all)
+    apply (rule Event\<^sub>c.etran.cases, simp_all)
     using guard_def body_def by (metis fstI sndI)
   with a1 a2 have a7 : "s\<^sub>a \<in> g\<^sub>a" 
     by (smt (verit, ccfv_SIG) CollectD case_prodE fst_conv rel_guard_eq_def snd_conv subsetD)
   with a5 have a8: "\<Gamma>\<^sub>a \<turnstile>\<^sub>a (BasicEvent (l\<^sub>a, g\<^sub>a, P\<^sub>a), s\<^sub>a, x\<^sub>a) -et-EvtEnt (BasicEvent (l\<^sub>a, g\<^sub>a, P\<^sub>a))\<sharp>k\<rightarrow> 
                    (AnonyEvent P\<^sub>a, s\<^sub>a, x\<^sub>a(k := BasicEvent (l\<^sub>a, g\<^sub>a, P\<^sub>a)))"
-    by (rule_tac InfoFlow\<^sub>a.EventEntry, simp_all add: body_def guard_def)
+    by (rule_tac Event\<^sub>a.EventEntry, simp_all add: body_def guard_def)
   from a2 a3 a6 a7 have "(s\<^sub>c, s\<^sub>a) \<in> \<eta>"
     by (simp add: rel_guard_and_def)
   with a0 have "(\<Gamma>\<^sub>c, (P\<^sub>c, s\<^sub>c), R\<^sub>c, G\<^sub>c) \<preceq>\<^sub>p \<^sub>(\<^sub>\<alpha>\<^sub>;\<^sub>\<zeta>\<^sub>;\<^sub>\<gamma>\<^sub>)  (\<Gamma>\<^sub>a, (P\<^sub>a, s\<^sub>a), R\<^sub>a, G\<^sub>a)"
@@ -250,12 +232,252 @@ theorem BasicEvent_Sound : "\<lbrakk>(\<Gamma>\<^sub>c, P\<^sub>c, R\<^sub>c, G\
   apply (rule conjI, clarsimp)
    apply (meson BasicEvent_Sound_lemma)
   apply (rule conjI, clarsimp)
-   apply (meson InfoFlow\<^sub>c.noevtent_notran0 act.distinct(1))
+   apply (meson Event\<^sub>c.noevtent_notran0 act.distinct(1))
   apply (rule conjI, clarsimp)
-   apply (meson InfoFlow\<^sub>c.noevtent_notran0 act.distinct(1))
+   apply (meson Event\<^sub>c.noevtent_notran0 act.distinct(1))
   by (meson Stable_def)
 
+coinductive es_sim :: "['Env\<^sub>c, ('l\<^sub>c,'k,'s\<^sub>c,'prog\<^sub>c) esconf, ('s\<^sub>c \<times> 's\<^sub>c) set, ('s\<^sub>c \<times> 's\<^sub>c) set, 
+                  ('s\<^sub>c \<times> 's\<^sub>a) set, 
+                  ('l\<^sub>c,'k,'s\<^sub>c,'prog\<^sub>c) event \<Rightarrow> ('l\<^sub>a,'k,'s\<^sub>a,'prog\<^sub>a) event, 
+                  ('l\<^sub>c,'k,'s\<^sub>c,'prog\<^sub>c) event \<Rightarrow> 'prog\<^sub>c \<Rightarrow> 'prog\<^sub>a option,
+                  'Env\<^sub>a, ('l\<^sub>a,'k,'s\<^sub>a,'prog\<^sub>a) esconf, ('s\<^sub>a \<times> 's\<^sub>a) set, ('s\<^sub>a \<times> 's\<^sub>a) set] \<Rightarrow> bool" 
+  ("'(_,_,_,_')/ \<preceq>\<^sub>e\<^sub>s \<^sub>'(\<^sub>_\<^sub>;\<^sub>_\<^sub>;\<^sub>_\<^sub>') /'(_,_,_,_')" [81,81,81,81,81,81,81,81,81,81,81] 100)
+  where rgsim : "\<lbrakk>(s\<^sub>c, s\<^sub>a) \<in> \<alpha>; 
+                  
+                  (\<forall>k.
 
+                  (\<forall>ec es\<^sub>c' x\<^sub>c'. (\<Gamma>\<^sub>c \<turnstile>\<^sub>c (es\<^sub>c, s\<^sub>c, x\<^sub>c) -es-((EvtEnt ec)\<sharp>k)\<rightarrow> (es\<^sub>c', s\<^sub>c, x\<^sub>c')) \<longrightarrow>(\<exists>ea es\<^sub>a' x\<^sub>a'. 
+                   (\<Gamma>\<^sub>a \<turnstile>\<^sub>a (es\<^sub>a, s\<^sub>a, x\<^sub>a) -es-((EvtEnt ea)\<sharp>k)\<rightarrow> (es\<^sub>a', s\<^sub>a, x\<^sub>a')) \<and> \<zeta> ec = ea \<and> 
+                    (\<Gamma>\<^sub>c, (es\<^sub>c', s\<^sub>c, x\<^sub>c'), R\<^sub>c, G\<^sub>c) \<preceq>\<^sub>e\<^sub>s \<^sub>(\<^sub>\<alpha>\<^sub>;\<^sub>\<zeta>\<^sub>;\<^sub>\<gamma>\<^sub>) (\<Gamma>\<^sub>a, (es\<^sub>a', s\<^sub>a, x\<^sub>a'), R\<^sub>a, G\<^sub>a))) \<and>
+
+                  (\<forall>Pc es\<^sub>c' s\<^sub>c'. (\<Gamma>\<^sub>c \<turnstile>\<^sub>c (es\<^sub>c, s\<^sub>c, x\<^sub>c) -es-((Cmd Pc)\<sharp>k)\<rightarrow> (es\<^sub>c', s\<^sub>c, x\<^sub>c')) \<and> \<gamma> (x\<^sub>c k) Pc = None \<longrightarrow>
+                  (s\<^sub>c, s\<^sub>c') \<in> G\<^sub>c \<and> (\<Gamma>\<^sub>c, (es\<^sub>c', s\<^sub>c', x\<^sub>c), R\<^sub>c, G\<^sub>c) \<preceq>\<^sub>e\<^sub>s \<^sub>(\<^sub>\<alpha>\<^sub>;\<^sub>\<zeta>\<^sub>;\<^sub>\<gamma>\<^sub>) (\<Gamma>\<^sub>a, (es\<^sub>a, s\<^sub>a, x\<^sub>a), R\<^sub>a, G\<^sub>a)) \<and>
+                  
+                  (\<forall>Pc es\<^sub>c' s\<^sub>c'. (\<Gamma>\<^sub>c \<turnstile>\<^sub>c (es\<^sub>c, s\<^sub>c, x\<^sub>c) -es-((Cmd Pc)\<sharp>k)\<rightarrow> (es\<^sub>c', s\<^sub>c, x\<^sub>c')) \<and> \<gamma> (x\<^sub>c k) Pc = Some Pa \<longrightarrow>
+                  (\<exists>es\<^sub>a' s\<^sub>a'. (\<Gamma>\<^sub>a \<turnstile>\<^sub>a (es\<^sub>a, s\<^sub>a, x\<^sub>a) -es-((Cmd Pa)\<sharp>k)\<rightarrow> (es\<^sub>a', s\<^sub>a', x\<^sub>a)) \<and> (s\<^sub>c, s\<^sub>c') \<in> G\<^sub>c \<and> (s\<^sub>a, s\<^sub>a') \<in> G\<^sub>a
+                  \<and> (\<Gamma>\<^sub>c, (es\<^sub>c', s\<^sub>c', x\<^sub>c), R\<^sub>c, G\<^sub>c) \<preceq>\<^sub>e\<^sub>s \<^sub>(\<^sub>\<alpha>\<^sub>;\<^sub>\<zeta>\<^sub>;\<^sub>\<gamma>\<^sub>) (\<Gamma>\<^sub>a, (es\<^sub>a, s\<^sub>a', x\<^sub>a), R\<^sub>a, G\<^sub>a)))
+
+                  ) ;
+
+                   (\<forall>s\<^sub>c' s\<^sub>a'. ((s\<^sub>c, s\<^sub>c'), (s\<^sub>a, s\<^sub>a')) \<in> ((R\<^sub>c, R\<^sub>a \<union> Id)\<^sub>\<alpha>) \<longrightarrow> 
+                     (\<Gamma>\<^sub>c, (es\<^sub>c, s\<^sub>c', x\<^sub>c'), R\<^sub>c, G\<^sub>c) \<preceq>\<^sub>e\<^sub>s \<^sub>(\<^sub>\<alpha>\<^sub>;\<^sub>\<zeta>\<^sub>;\<^sub>\<gamma>\<^sub>) (\<Gamma>\<^sub>a, (es\<^sub>a, s\<^sub>a', x\<^sub>a'), R\<^sub>a, G\<^sub>a))      
+                  \<rbrakk> \<Longrightarrow> (\<Gamma>\<^sub>c, (es\<^sub>c, s\<^sub>c, x\<^sub>c), R\<^sub>c, G\<^sub>c) \<preceq>\<^sub>e\<^sub>s \<^sub>(\<^sub>\<alpha>\<^sub>;\<^sub>\<zeta>\<^sub>;\<^sub>\<gamma>\<^sub>) (\<Gamma>\<^sub>a, (es\<^sub>a, s\<^sub>a, x\<^sub>a), R\<^sub>a, G\<^sub>a)"
+
+inductive pes_sim :: "['Env\<^sub>c, ('l\<^sub>c,'k,'s\<^sub>c,'prog\<^sub>c) pesconf, 
+                  ('s\<^sub>c \<times> 's\<^sub>a) set, 
+                  ('l\<^sub>c,'k,'s\<^sub>c,'prog\<^sub>c) event \<Rightarrow> ('l\<^sub>a,'k,'s\<^sub>a,'prog\<^sub>a) event, 
+                  ('l\<^sub>c,'k,'s\<^sub>c,'prog\<^sub>c) event \<Rightarrow> 'prog\<^sub>c \<Rightarrow> 'prog\<^sub>a option,
+                  'Env\<^sub>a, ('l\<^sub>a,'k,'s\<^sub>a,'prog\<^sub>a) pesconf] \<Rightarrow> bool" 
+  ("'(_,_')/ \<preceq>\<^sub>p\<^sub>e\<^sub>s \<^sub>'(\<^sub>_\<^sub>;\<^sub>_\<^sub>;\<^sub>_\<^sub>') /'(_,_')" [81,81,81,81,81,81,81] 100)
+  where rgsim : "\<lbrakk>(s\<^sub>c, s\<^sub>a) \<in> \<alpha>; 
+                  
+                  (\<forall>ec pes\<^sub>c' x\<^sub>c' k. (\<Gamma>\<^sub>c \<turnstile>\<^sub>c (pes\<^sub>c, s\<^sub>c, x\<^sub>c) -pes-((EvtEnt ec)\<sharp>k)\<rightarrow> (pes\<^sub>c', s\<^sub>c, x\<^sub>c')) \<longrightarrow>(\<exists>ea pes\<^sub>a' x\<^sub>a'. 
+                  (\<Gamma>\<^sub>a \<turnstile>\<^sub>a (pes\<^sub>a, s\<^sub>a, x\<^sub>a) -pes-((EvtEnt ea)\<sharp>k)\<rightarrow> (pes\<^sub>a', s\<^sub>a, x\<^sub>a')) \<and> \<eta> ec = ea \<and> 
+                  (\<Gamma>\<^sub>c, (pes\<^sub>c', s\<^sub>c, x\<^sub>c')) \<preceq>\<^sub>p\<^sub>e\<^sub>s \<^sub>(\<^sub>\<alpha>\<^sub>;\<^sub>\<eta>\<^sub>;\<^sub>\<kappa>\<^sub>) (\<Gamma>\<^sub>a, (pes\<^sub>a', s\<^sub>a, x\<^sub>a'))));
+
+                  (\<forall>Pc pes\<^sub>c' s\<^sub>c' k. (\<Gamma>\<^sub>c \<turnstile>\<^sub>c (pes\<^sub>c, s\<^sub>c, x\<^sub>c) -pes-((Cmd Pc)\<sharp>k)\<rightarrow> (pes\<^sub>c', s\<^sub>c', x\<^sub>c)) \<and> \<kappa> (x\<^sub>c k) Pc = None \<longrightarrow>
+                  (\<Gamma>\<^sub>c, (pes\<^sub>c', s\<^sub>c', x\<^sub>c)) \<preceq>\<^sub>p\<^sub>e\<^sub>s \<^sub>(\<^sub>\<alpha>\<^sub>;\<^sub>\<eta>\<^sub>;\<^sub>\<kappa>\<^sub>) (\<Gamma>\<^sub>a, (pes\<^sub>a, s\<^sub>a, x\<^sub>a)));
+
+                  (\<forall>Pc pes\<^sub>c' s\<^sub>c' k Pa. (\<Gamma>\<^sub>c \<turnstile>\<^sub>c (pes\<^sub>c, s\<^sub>c, x\<^sub>c) -pes-((Cmd Pc)\<sharp>k)\<rightarrow> (pes\<^sub>c', s\<^sub>c', x\<^sub>c)) \<and> \<kappa> (x\<^sub>c k) Pc = Some Pa \<longrightarrow>
+                  (\<exists>pes\<^sub>a' s\<^sub>a'. (\<Gamma>\<^sub>a \<turnstile>\<^sub>a (pes\<^sub>a, s\<^sub>a, x\<^sub>a) -pes-((Cmd Pa)\<sharp>k)\<rightarrow> (pes\<^sub>a', s\<^sub>a', x\<^sub>a)) \<and> \<eta> (x\<^sub>c k) = (x\<^sub>a k)
+                  \<and> (\<Gamma>\<^sub>c, (pes\<^sub>c', s\<^sub>c', x\<^sub>c)) \<preceq>\<^sub>p\<^sub>e\<^sub>s \<^sub>(\<^sub>\<alpha>\<^sub>;\<^sub>\<eta>\<^sub>;\<^sub>\<kappa>\<^sub>) (\<Gamma>\<^sub>a, (pes\<^sub>a', s\<^sub>a', x\<^sub>a)))) 
+     
+                  \<rbrakk> \<Longrightarrow> (\<Gamma>\<^sub>c, (pes\<^sub>c, s\<^sub>c, x\<^sub>c)) \<preceq>\<^sub>p\<^sub>e\<^sub>s \<^sub>(\<^sub>\<alpha>\<^sub>;\<^sub>\<eta>\<^sub>;\<^sub>\<kappa>\<^sub>) (\<Gamma>\<^sub>a, (pes\<^sub>a, s\<^sub>a, x\<^sub>a))"
+
+
+
+lemma KKV: "\<lbrakk>\<forall>k. (\<Gamma>\<^sub>c, (pes\<^sub>c k, s\<^sub>c, x\<^sub>c), (R\<^sub>c k), (G\<^sub>c k)) \<preceq>\<^sub>e\<^sub>s \<^sub>(\<^sub>\<alpha>\<^sub>;\<^sub>\<eta>\<^sub>;\<^sub>\<kappa>\<^sub>) (\<Gamma>\<^sub>a, (pes\<^sub>a k, s\<^sub>a, x\<^sub>a), (R\<^sub>a k), (G\<^sub>a k));
+             \<forall>i j. i \<noteq> j \<longrightarrow> G\<^sub>c i \<subseteq> R\<^sub>c j \<and> G\<^sub>a i \<subseteq> R\<^sub>a j\<rbrakk> \<Longrightarrow> (\<Gamma>\<^sub>c, (pes\<^sub>c, s\<^sub>c, x\<^sub>c)) \<preceq>\<^sub>p\<^sub>e\<^sub>s \<^sub>(\<^sub>\<alpha>\<^sub>;\<^sub>\<eta>\<^sub>;\<^sub>\<kappa>\<^sub>) (\<Gamma>\<^sub>a, (pes\<^sub>a, s\<^sub>a, x\<^sub>a))"
+(*
+inductive None_event :: "('l\<^sub>c, 'k, 's\<^sub>c, 'prog\<^sub>c) event \<Rightarrow> ('s\<^sub>c \<times> 's\<^sub>a) set \<Rightarrow> ('s\<^sub>c \<times> 's\<^sub>a) set \<Rightarrow> bool"
+  where "None_event e \<xi> \<gamma> = (\<forall>s\<^sub>c s\<^sub>a. 
+         )"
+*)
+end
+ 
+
+locale PiCore_RGSim = 
+       Sim: PiCore_Sim ptran\<^sub>c petran\<^sub>c fin_com\<^sub>c ptran\<^sub>a petran\<^sub>a fin_com\<^sub>a +
+       InfoFlow\<^sub>c: InfoFlow ptran\<^sub>c petran\<^sub>c fin_com\<^sub>c \<Gamma>\<^sub>c C0\<^sub>c step\<^sub>c interference\<^sub>c vpeq\<^sub>c obs\<^sub>c dome\<^sub>c +
+       InfoFlow\<^sub>a: InfoFlow ptran\<^sub>a petran\<^sub>a fin_com\<^sub>a \<Gamma>\<^sub>a C0\<^sub>a step\<^sub>a interference\<^sub>a vpeq\<^sub>a obs\<^sub>a dome\<^sub>a
+  for ptran\<^sub>c :: "'Env\<^sub>c \<Rightarrow> (('prog\<^sub>c \<times> 's\<^sub>c) \<times> 'prog\<^sub>c \<times> 's\<^sub>c) set" 
+  and petran\<^sub>c :: "'Env\<^sub>c \<Rightarrow> 'prog\<^sub>c \<times> 's\<^sub>c \<Rightarrow> 'prog\<^sub>c \<times> 's\<^sub>c \<Rightarrow> bool" 
+  and fin_com\<^sub>c :: "'prog\<^sub>c"
+  and \<Gamma>\<^sub>c :: "'Env\<^sub>c"
+  and C0\<^sub>c  :: "('l\<^sub>c,'k,'s\<^sub>c,'prog\<^sub>c) pesconf"
+  and step\<^sub>c :: "('l\<^sub>c,'k,'s\<^sub>c,'prog\<^sub>c, 'd) action \<Rightarrow> (('l\<^sub>c,'k,'s\<^sub>c,'prog\<^sub>c) pesconf \<times> ('l\<^sub>c,'k,'s\<^sub>c,'prog\<^sub>c) pesconf) set"
+  and interference\<^sub>c :: "'d \<Rightarrow> 'd \<Rightarrow> bool" 
+  and vpeq\<^sub>c :: "'s\<^sub>c \<Rightarrow> 'd \<Rightarrow> 's\<^sub>c \<Rightarrow> bool" ("(_ \<sim>\<^sub>c_\<sim>\<^sub>c _)" [70,69,70] 60)
+  and obs\<^sub>c :: "'s\<^sub>c \<Rightarrow> 'd \<Rightarrow> 'o\<^sub>c" 
+  and dome\<^sub>c :: "'s\<^sub>c \<Rightarrow> ('l\<^sub>c, 'k, 's\<^sub>c, 'prog\<^sub>c) event \<Rightarrow> 'd"
+  and ptran\<^sub>a :: "'Env\<^sub>a \<Rightarrow> (('prog\<^sub>a \<times> 's\<^sub>a) \<times> 'prog\<^sub>a \<times> 's\<^sub>a) set"
+  and petran\<^sub>a :: "'Env\<^sub>a \<Rightarrow> 'prog\<^sub>a \<times> 's\<^sub>a \<Rightarrow> 'prog\<^sub>a \<times> 's\<^sub>a \<Rightarrow> bool" 
+  and fin_com\<^sub>a :: "'prog\<^sub>a"
+  and \<Gamma>\<^sub>a :: "'Env\<^sub>a"
+  and C0\<^sub>a :: "('l\<^sub>a, 'k, 's\<^sub>a, 'prog\<^sub>a) pesconf"
+  and step\<^sub>a :: "('l\<^sub>a,'k,'s\<^sub>a,'prog\<^sub>a, 'd) action \<Rightarrow> (('l\<^sub>a,'k,'s\<^sub>a,'prog\<^sub>a) pesconf \<times> ('l\<^sub>a,'k,'s\<^sub>a,'prog\<^sub>a) pesconf) set" 
+  and interference\<^sub>a :: "'d \<Rightarrow> 'd \<Rightarrow> bool" 
+  and vpeq\<^sub>a ::  "'s\<^sub>a \<Rightarrow> 'd \<Rightarrow> 's\<^sub>a \<Rightarrow> bool" ("(_ \<sim>\<^sub>a_\<sim>\<^sub>a _)" [70,69,70] 60)
+  and obs\<^sub>a :: "'s\<^sub>a \<Rightarrow> 'd \<Rightarrow> 'o\<^sub>a" 
+  and dome\<^sub>a :: "'s\<^sub>a \<Rightarrow> ('l\<^sub>a, 'k, 's\<^sub>a, 'prog\<^sub>a) event \<Rightarrow> 'd" +
+fixes \<alpha> :: "('s\<^sub>c \<times> 's\<^sub>a) set"
+  and \<eta> :: "('l\<^sub>c,'k,'s\<^sub>c,'prog\<^sub>c) event \<Rightarrow> ('l\<^sub>a,'k,'s\<^sub>a,'prog\<^sub>a) event"
+  and \<kappa> :: "('l\<^sub>c,'k,'s\<^sub>c,'prog\<^sub>c) event \<Rightarrow> 'prog\<^sub>c \<Rightarrow> 'prog\<^sub>a option"
+assumes
+  init_sim : "(\<Gamma>\<^sub>c, C0\<^sub>c) \<preceq>\<^sub>p\<^sub>e\<^sub>s \<^sub>(\<^sub>\<alpha>\<^sub>;\<^sub>\<eta>\<^sub>;\<^sub>\<kappa>\<^sub>) (\<Gamma>\<^sub>a, C0\<^sub>a)" and
+  dom_sim : "\<lbrakk>(s\<^sub>c, s\<^sub>a) \<in> \<alpha>; \<eta> e\<^sub>c = e\<^sub>a \<rbrakk> \<Longrightarrow> dome\<^sub>c s\<^sub>c e\<^sub>c = dome\<^sub>a s\<^sub>a e\<^sub>a" and
+  intefere_same : "interference\<^sub>c  = interference\<^sub>a" and
+  sim_state_ifs : "\<lbrakk>(s\<^sub>c, s\<^sub>a) \<in> \<alpha>; (t\<^sub>c, t\<^sub>a) \<in> \<alpha>\<rbrakk> \<Longrightarrow> s\<^sub>a \<sim>\<^sub>a d \<sim>\<^sub>a t\<^sub>a = s\<^sub>c \<sim>\<^sub>c d \<sim>\<^sub>c t\<^sub>c"
+begin
+
+definition sim_s :: "('l\<^sub>c,'k,'s\<^sub>c,'prog\<^sub>c) pesconf \<Rightarrow> ('l\<^sub>a, 'k, 's\<^sub>a, 'prog\<^sub>a) pesconf \<Rightarrow> bool" ("(_ \<sim> _)" [70,70] 60)
+  where "C\<^sub>c \<sim> C\<^sub>a = (\<Gamma>\<^sub>c, C\<^sub>c) \<preceq>\<^sub>p\<^sub>e\<^sub>s \<^sub>(\<^sub>\<alpha>\<^sub>;\<^sub>\<eta>\<^sub>;\<^sub>\<kappa>\<^sub>) (\<Gamma>\<^sub>a, C\<^sub>a)"
+
+fun sim_a :: "('l\<^sub>c, 'k, 's\<^sub>c, 'prog\<^sub>c, 'd) action \<Rightarrow> ('l\<^sub>a, 'k, 's\<^sub>a, 'prog\<^sub>a, 'd) action option"
+  where "sim_a \<lparr>actk = \<lparr>Act = Cmd P\<^sub>c, K = k\<rparr>, eventof = e\<^sub>c, domain = d\<rparr> = 
+         (if (\<kappa> e\<^sub>c P\<^sub>c = None) then None 
+         else Some (let e\<^sub>a = \<eta> e\<^sub>c; P\<^sub>a = the (\<kappa> e\<^sub>c P\<^sub>c) in 
+              \<lparr>actk = \<lparr>Act = Cmd P\<^sub>a, K = k\<rparr>, eventof = e\<^sub>a, domain = d\<rparr>))" |
+        "sim_a \<lparr>actk = \<lparr>Act = EvtEnt e\<^sub>c, K = k\<rparr>, eventof = ec, domain = d\<rparr> = 
+         Some \<lparr>actk = \<lparr>Act = EvtEnt (\<eta> e\<^sub>c), K = k\<rparr>, eventof = \<eta> e\<^sub>c, domain = d\<rparr>"
+
+lemma dom_refine : "sim_a a\<^sub>c = Some a\<^sub>a \<Longrightarrow> domain a\<^sub>c = domain a\<^sub>a"
+  apply (case_tac a\<^sub>c, case_tac actk, case_tac Act, simp_all)
+   apply (metis action.select_convs(3) option.discI option.inject)
+  by (metis action.select_convs(3))
+
+lemma none_refine: "\<lbrakk>sim_a a\<^sub>c = None; C\<^sub>c \<sim> C\<^sub>a; (C\<^sub>c, C\<^sub>c') \<in> step\<^sub>c a\<^sub>c\<rbrakk> \<Longrightarrow> C\<^sub>c' \<sim> C\<^sub>a"
+proof-
+  assume a0: "sim_a a\<^sub>c = None"
+     and a1: "C\<^sub>c \<sim> C\<^sub>a"
+     and a2: "(C\<^sub>c, C\<^sub>c') \<in> step\<^sub>c a\<^sub>c"
+
+  from a0 have "is_Cmd_act (Act (actk a\<^sub>c))"
+    by (metis act.exhaust action.surjective actk.surjective is_Cmd_act.simps(1) old.unit.exhaust option.distinct(1) sim_a.simps(2))
+  then obtain P\<^sub>c k e\<^sub>c d where a3: "a\<^sub>c = \<lparr>actk = \<lparr>Act = Cmd P\<^sub>c, K = k\<rparr>, eventof = e\<^sub>c, domain = d\<rparr>"
+    by (metis act.exhaust action.surjective actk.surjective is_Cmd_act.simps(2) old.unit.exhaust)
+  with a0 have a4: "\<kappa> e\<^sub>c P\<^sub>c = None"
+    by (metis option.discI sim_a.simps(1))
+
+  obtain pes\<^sub>c s\<^sub>c x\<^sub>c pes\<^sub>c' s\<^sub>c' x\<^sub>c' where a5: "C\<^sub>c = (pes\<^sub>c ,s\<^sub>c ,x\<^sub>c) \<and> C\<^sub>c' = (pes\<^sub>c', s\<^sub>c', x\<^sub>c')" 
+    by (meson Sim.Event\<^sub>c.pesconf_trip)
+  with a2 a3 have a6: "(\<Gamma>\<^sub>c \<turnstile>\<^sub>c (pes\<^sub>c ,s\<^sub>c ,x\<^sub>c) -pes-(Cmd P\<^sub>c)\<sharp>k \<rightarrow> (pes\<^sub>c', s\<^sub>c', x\<^sub>c')) \<and> (x\<^sub>c k = e\<^sub>c)"
+    by (simp add: InfoFlow\<^sub>c.step_def get_actk_def getx_def)
+  then have a7: "x\<^sub>c = x\<^sub>c'"
+    by (meson Sim.Event\<^sub>c.act_in_pes_notchgstate)
+
+  with a1 a4 a5 a6 show ?thesis
+    apply (simp add: sim_s_def)
+    apply (erule Sim.pes_sim.cases, simp)
+    by (metis Sim.Event\<^sub>c.pesconf_trip snd_conv)
+qed
+
+lemma action_refine: "\<lbrakk>sim_a a\<^sub>c = Some a\<^sub>a; C\<^sub>c \<sim> C\<^sub>a; (C\<^sub>c, C\<^sub>c') \<in> step\<^sub>c a\<^sub>c\<rbrakk> \<Longrightarrow> \<exists>C\<^sub>a'. C\<^sub>c' \<sim> C\<^sub>a' \<and> (C\<^sub>a, C\<^sub>a') \<in> step\<^sub>a a\<^sub>a"
+proof-
+  assume a0: "sim_a a\<^sub>c = Some a\<^sub>a"
+     and a1: "C\<^sub>c \<sim> C\<^sub>a"
+     and a2: "(C\<^sub>c, C\<^sub>c') \<in> step\<^sub>c a\<^sub>c"
+  then have "\<exists>C\<^sub>a'. C\<^sub>c' \<sim> C\<^sub>a' \<and> (C\<^sub>a, C\<^sub>a') \<in> step\<^sub>a a\<^sub>a"
+  proof(case_tac "Act (actk a\<^sub>c)")
+    fix P\<^sub>c
+    assume "Act (actk a\<^sub>c) = Cmd P\<^sub>c"
+    then obtain k e\<^sub>c d where b0: "a\<^sub>c = \<lparr>actk = \<lparr>Act = Cmd P\<^sub>c, K = k\<rparr>, eventof = e\<^sub>c, domain = d\<rparr>"
+      by (metis action.surjective actk.surjective old.unit.exhaust)
+    with a0 have "\<exists>P\<^sub>a. \<kappa> e\<^sub>c P\<^sub>c = Some P\<^sub>a"
+      by (metis option.discI option.exhaust_sel sim_a.simps(1))
+    then obtain P\<^sub>a where b1: "\<kappa> e\<^sub>c P\<^sub>c = Some P\<^sub>a" by auto
+    with a0 b0 have b2: "a\<^sub>a = \<lparr>actk = \<lparr>Act = Cmd P\<^sub>a, K = k\<rparr>, eventof = \<eta> e\<^sub>c, domain = d\<rparr>" by auto
+
+    obtain pes\<^sub>c s\<^sub>c x\<^sub>c pes\<^sub>c' s\<^sub>c' x\<^sub>c' where b3: "C\<^sub>c = (pes\<^sub>c ,s\<^sub>c ,x\<^sub>c) \<and> C\<^sub>c' = (pes\<^sub>c', s\<^sub>c', x\<^sub>c')" 
+      by (meson Sim.Event\<^sub>c.pesconf_trip)
+    with a2 b0 have b4: "(\<Gamma>\<^sub>c \<turnstile>\<^sub>c (pes\<^sub>c ,s\<^sub>c ,x\<^sub>c) -pes-(Cmd P\<^sub>c)\<sharp>k \<rightarrow> (pes\<^sub>c', s\<^sub>c', x\<^sub>c')) \<and> (x\<^sub>c k = e\<^sub>c) \<and> (dome\<^sub>c s\<^sub>c e\<^sub>c = d)"
+      apply (simp add: InfoFlow\<^sub>c.step_def get_actk_def gets_def getx_def)
+      by blast
+    obtain pes\<^sub>a s\<^sub>a x\<^sub>a where b5: "C\<^sub>a = (pes\<^sub>a, s\<^sub>a, x\<^sub>a)" by (meson Sim.Event\<^sub>c.pesconf_trip)
+    with a1 b1 b3 b4 have "\<exists>pes\<^sub>a' s\<^sub>a'. (\<Gamma>\<^sub>a \<turnstile>\<^sub>a (pes\<^sub>a, s\<^sub>a, x\<^sub>a) -pes-((Cmd P\<^sub>a)\<sharp>k)\<rightarrow> (pes\<^sub>a', s\<^sub>a', x\<^sub>a))
+    \<and> \<eta> (x\<^sub>c k) = (x\<^sub>a k) \<and> (\<Gamma>\<^sub>c, (pes\<^sub>c', s\<^sub>c', x\<^sub>c)) \<preceq>\<^sub>p\<^sub>e\<^sub>s \<^sub>(\<^sub>\<alpha>\<^sub>;\<^sub>\<eta>\<^sub>;\<^sub>\<kappa>\<^sub>) (\<Gamma>\<^sub>a, (pes\<^sub>a', s\<^sub>a', x\<^sub>a))"
+      apply (simp add: sim_s_def)
+      apply (erule Sim.pes_sim.cases, simp)
+      by (metis Sim.Event\<^sub>c.act_in_pes_notchgstate)
+    then obtain pes\<^sub>a' s\<^sub>a' where b6: "(\<Gamma>\<^sub>a \<turnstile>\<^sub>a (pes\<^sub>a, s\<^sub>a, x\<^sub>a) -pes-((Cmd P\<^sub>a)\<sharp>k)\<rightarrow> (pes\<^sub>a', s\<^sub>a', x\<^sub>a))
+    \<and> \<eta> (x\<^sub>c k) = (x\<^sub>a k) \<and> (\<Gamma>\<^sub>c, (pes\<^sub>c', s\<^sub>c', x\<^sub>c)) \<preceq>\<^sub>p\<^sub>e\<^sub>s \<^sub>(\<^sub>\<alpha>\<^sub>;\<^sub>\<eta>\<^sub>;\<^sub>\<kappa>\<^sub>) (\<Gamma>\<^sub>a, (pes\<^sub>a', s\<^sub>a', x\<^sub>a))" by auto
+
+    from a1 b3 b5 have "(s\<^sub>c, s\<^sub>a) \<in> \<alpha>"
+      by (simp add: Sim.pes_sim_init sim_s_def)      
+    with b2 b3 b4 b5 b6 have "dome\<^sub>a (gets C\<^sub>a) (eventof a\<^sub>a) = domain a\<^sub>a"
+      apply (simp add: gets_def)
+      apply (rule_tac s = "dome\<^sub>c s\<^sub>c e\<^sub>c" in trans)
+      using dom_sim apply auto[1]
+      using b5 by auto
+    with b2 b4 b5 b6 have "actk a\<^sub>a = ((Cmd P\<^sub>a)\<sharp>k) \<and> eventof a\<^sub>a = (getx C\<^sub>a) k \<and> dome\<^sub>a (gets C\<^sub>a) (eventof a\<^sub>a) = domain a\<^sub>a"
+      by (metis Sim.Event\<^sub>a.act_in_pes_notchgstate Sim.Event\<^sub>a.event_axioms action.select_convs(1) 
+         action.select_convs(2)  event.pesconf_trip get_actk_def)
+    with b5 b6 have "(C\<^sub>a, (pes\<^sub>a', s\<^sub>a', x\<^sub>a)) \<in> step\<^sub>a a\<^sub>a"
+      using InfoFlow\<^sub>a.step_def by fastforce
+    with b3 b4 b6 show ?thesis
+      by (metis Sim.Event\<^sub>c.event_axioms event.act_in_pes_notchgstate sim_s_def)
+  next
+    fix e\<^sub>c
+    assume "Act (actk a\<^sub>c) = EvtEnt e\<^sub>c"
+    then obtain k ec d where b0: "a\<^sub>c = \<lparr>actk = \<lparr>Act = EvtEnt e\<^sub>c, K = k\<rparr>, eventof = ec, domain = d\<rparr>"
+      by (metis action.surjective actk.surjective old.unit.exhaust)
+    with a0 have b1: "a\<^sub>a = \<lparr>actk = \<lparr>Act = EvtEnt (\<eta> e\<^sub>c), K = k\<rparr>, eventof = \<eta> e\<^sub>c, domain = d\<rparr>"
+      by force
+    obtain pes\<^sub>c s\<^sub>c x\<^sub>c pes\<^sub>c' s\<^sub>c' x\<^sub>c' where b3: "C\<^sub>c = (pes\<^sub>c ,s\<^sub>c ,x\<^sub>c) \<and> C\<^sub>c' = (pes\<^sub>c', s\<^sub>c', x\<^sub>c')" 
+      by (meson Sim.Event\<^sub>c.pesconf_trip)
+    with b0 a2 have b4: "(\<Gamma>\<^sub>c \<turnstile>\<^sub>c (pes\<^sub>c ,s\<^sub>c ,x\<^sub>c) -pes-(EvtEnt e\<^sub>c)\<sharp>k \<rightarrow> (pes\<^sub>c', s\<^sub>c', x\<^sub>c')) \<and> ec = e\<^sub>c \<and> dome\<^sub>c s\<^sub>c e\<^sub>c = d"
+      by (simp add: InfoFlow\<^sub>c.step_def get_actk_def gets_def getx_def)
+    then have b5: "s\<^sub>c = s\<^sub>c'"
+      by (metis Sim.Event\<^sub>c.evtent_in_pes_notchgstate)
+    obtain pes\<^sub>a s\<^sub>a x\<^sub>a where b6: "C\<^sub>a = (pes\<^sub>a, s\<^sub>a, x\<^sub>a)" by (meson Sim.Event\<^sub>c.pesconf_trip)
+    with a1 b3 b4 have "\<exists>e\<^sub>a pes\<^sub>a' x\<^sub>a'. (\<Gamma>\<^sub>a \<turnstile>\<^sub>a (pes\<^sub>a, s\<^sub>a, x\<^sub>a) -pes-((EvtEnt e\<^sub>a)\<sharp>k)\<rightarrow> (pes\<^sub>a', s\<^sub>a, x\<^sub>a'))
+    \<and> \<eta> e\<^sub>c = e\<^sub>a \<and> (\<Gamma>\<^sub>c, (pes\<^sub>c', s\<^sub>c, x\<^sub>c')) \<preceq>\<^sub>p\<^sub>e\<^sub>s \<^sub>(\<^sub>\<alpha>\<^sub>;\<^sub>\<eta>\<^sub>;\<^sub>\<kappa>\<^sub>) (\<Gamma>\<^sub>a, (pes\<^sub>a', s\<^sub>a, x\<^sub>a'))"
+      apply (simp add: sim_s_def)
+      apply (erule Sim.pes_sim.cases, simp)
+      by (metis Sim.Event\<^sub>c.evtent_in_pes_notchgstate)
+    then obtain pes\<^sub>a' x\<^sub>a' where b7: "(\<Gamma>\<^sub>a \<turnstile>\<^sub>a (pes\<^sub>a, s\<^sub>a, x\<^sub>a) -pes-((EvtEnt (\<eta> e\<^sub>c))\<sharp>k)\<rightarrow> (pes\<^sub>a', s\<^sub>a, x\<^sub>a'))
+     \<and> (\<Gamma>\<^sub>c, (pes\<^sub>c', s\<^sub>c, x\<^sub>c')) \<preceq>\<^sub>p\<^sub>e\<^sub>s \<^sub>(\<^sub>\<alpha>\<^sub>;\<^sub>\<eta>\<^sub>;\<^sub>\<kappa>\<^sub>) (\<Gamma>\<^sub>a, (pes\<^sub>a', s\<^sub>a, x\<^sub>a'))" by auto
+
+    then have "(s\<^sub>c, s\<^sub>a) \<in> \<alpha>"
+      using Sim.pes_sim_init by blast
+    with b1 b4 b6 have "dome\<^sub>a (gets C\<^sub>a) (\<eta> e\<^sub>c) = domain a\<^sub>a"
+      by (metis action.select_convs(3) dom_sim fst_conv gets_def snd_conv)
+    with b1 have "actk a\<^sub>a = (EvtEnt (\<eta> e\<^sub>c))\<sharp>k \<and> eventof a\<^sub>a = \<eta> e\<^sub>c \<and> dome\<^sub>a (gets C\<^sub>a) (\<eta> e\<^sub>c) = domain a\<^sub>a"
+      by (simp add: get_actk_def)
+    with b6 b7 have "(C\<^sub>a, (pes\<^sub>a', s\<^sub>a, x\<^sub>a')) \<in> step\<^sub>a a\<^sub>a"
+      using InfoFlow\<^sub>a.step_def by auto
+    with b3 b5 b7 show ?thesis
+      using  sim_s_def by blast
+  qed
+
+  then show ?thesis by auto
+qed   
+
+lemma sim_ifs : "\<lbrakk>C\<^sub>c \<sim> C\<^sub>a; T\<^sub>c \<sim> T\<^sub>a\<rbrakk> \<Longrightarrow>  (gets C\<^sub>a) \<sim>\<^sub>a d \<sim>\<^sub>a (gets T\<^sub>a) = (gets C\<^sub>c) \<sim>\<^sub>c d \<sim>\<^sub>c (gets T\<^sub>c)"
+  by (metis (mono_tags, lifting) Sim.Event\<^sub>c.pesconf_trip Sim.pes_sim_init sim_s_def sim_state_ifs)
+
+interpretation PiCore_Refine ptran\<^sub>c petran\<^sub>c fin_com\<^sub>c \<Gamma>\<^sub>c C0\<^sub>c step\<^sub>c interference\<^sub>c vpeq\<^sub>c obs\<^sub>c dome\<^sub>c
+                             ptran\<^sub>a petran\<^sub>a fin_com\<^sub>a \<Gamma>\<^sub>a C0\<^sub>a step\<^sub>a interference\<^sub>a vpeq\<^sub>a obs\<^sub>a dome\<^sub>a
+                             sim_s sim_a
+proof
+  show "C0\<^sub>c \<sim> C0\<^sub>a"
+    by (simp add: init_sim sim_s_def)
+  show "\<And>a\<^sub>c a\<^sub>a C\<^sub>c C\<^sub>a C\<^sub>c'. sim_a a\<^sub>c = Some a\<^sub>a \<Longrightarrow> InfoFlow\<^sub>c.reachablec0 C\<^sub>c \<Longrightarrow> C\<^sub>c \<sim> C\<^sub>a \<Longrightarrow> 
+        (C\<^sub>c, C\<^sub>c') \<in> step\<^sub>c a\<^sub>c \<Longrightarrow> \<exists>C\<^sub>a'. C\<^sub>c' \<sim> C\<^sub>a' \<and> (C\<^sub>a, C\<^sub>a') \<in> step\<^sub>a a\<^sub>a"
+    using action_refine by auto
+  show "\<And>a\<^sub>c C\<^sub>c C\<^sub>a C\<^sub>c'. sim_a a\<^sub>c = None \<Longrightarrow> InfoFlow\<^sub>c.reachablec0 C\<^sub>c \<Longrightarrow> C\<^sub>c \<sim> C\<^sub>a \<Longrightarrow> (C\<^sub>c, C\<^sub>c') \<in> step\<^sub>c a\<^sub>c 
+        \<Longrightarrow> C\<^sub>c' \<sim> C\<^sub>a"
+    using none_refine by blast
+  show "interference\<^sub>c = interference\<^sub>a"
+    by (simp add: intefere_same)
+  show "\<And>a\<^sub>c a\<^sub>a. sim_a a\<^sub>c = Some a\<^sub>a \<longrightarrow> domain a\<^sub>c = domain a\<^sub>a"
+    using dom_refine by presburger
+  show "\<And>C\<^sub>c C\<^sub>a T\<^sub>c T\<^sub>a d. C\<^sub>c \<sim> C\<^sub>a \<Longrightarrow> T\<^sub>c \<sim> T\<^sub>a \<Longrightarrow> gets C\<^sub>a \<sim>\<^sub>ad\<sim>\<^sub>a gets T\<^sub>a = gets C\<^sub>c \<sim>\<^sub>cd\<sim>\<^sub>c gets T\<^sub>c "
+    by (simp add: sim_ifs)
+qed
+
+end
 
 end
 
