PiCore_Refine.thy
@@ -2,12 +2,15 @@ theory PiCore_Refine
   imports PiCore_IFS Refinement
 begin
 
+print_locale InfoFlow
+
 locale PiCore_Refine =
-  InfoFlow\<^sub>c: InfoFlow ptran\<^sub>c petran\<^sub>c fin_com\<^sub>c C0\<^sub>c step\<^sub>c interference\<^sub>c vpeq\<^sub>c obs\<^sub>c dome\<^sub>c +
-  InfoFlow\<^sub>a: InfoFlow ptran\<^sub>a petran\<^sub>a fin_com\<^sub>a C0\<^sub>a step\<^sub>a interference\<^sub>a vpeq\<^sub>a obs\<^sub>a dome\<^sub>a
+  InfoFlow\<^sub>c: InfoFlow ptran\<^sub>c petran\<^sub>c fin_com\<^sub>c \<Gamma>\<^sub>c C0\<^sub>c step\<^sub>c interference\<^sub>c vpeq\<^sub>c obs\<^sub>c dome\<^sub>c +
+  InfoFlow\<^sub>a: InfoFlow ptran\<^sub>a petran\<^sub>a fin_com\<^sub>a \<Gamma>\<^sub>a C0\<^sub>a step\<^sub>a interference\<^sub>a vpeq\<^sub>a obs\<^sub>a dome\<^sub>a
   for ptran\<^sub>c :: "'Env\<^sub>c \<Rightarrow> (('prog\<^sub>c \<times> 's\<^sub>c) \<times> 'prog\<^sub>c \<times> 's\<^sub>c) set" 
   and petran\<^sub>c :: "'Env\<^sub>c \<Rightarrow> 'prog\<^sub>c \<times> 's\<^sub>c \<Rightarrow> 'prog\<^sub>c \<times> 's\<^sub>c \<Rightarrow> bool" 
   and fin_com\<^sub>c :: "'prog\<^sub>c"
+  and \<Gamma>\<^sub>c :: "'Env\<^sub>c"
   and C0\<^sub>c  :: "('l\<^sub>c,'k\<^sub>c,'s\<^sub>c,'prog\<^sub>c) pesconf"
   and step\<^sub>c :: "('l\<^sub>c,'k\<^sub>c,'s\<^sub>c,'prog\<^sub>c, 'd) action \<Rightarrow> (('l\<^sub>c,'k\<^sub>c,'s\<^sub>c,'prog\<^sub>c) pesconf \<times> ('l\<^sub>c,'k\<^sub>c,'s\<^sub>c,'prog\<^sub>c) pesconf) set"
   and interference\<^sub>c :: "'d \<Rightarrow> 'd \<Rightarrow> bool" 
@@ -17,6 +20,7 @@ locale PiCore_Refine =
   and ptran\<^sub>a :: "'Env\<^sub>a \<Rightarrow> (('prog\<^sub>a \<times> 's\<^sub>a) \<times> 'prog\<^sub>a \<times> 's\<^sub>a) set"
   and petran\<^sub>a :: "'Env\<^sub>a \<Rightarrow> 'prog\<^sub>a \<times> 's\<^sub>a \<Rightarrow> 'prog\<^sub>a \<times> 's\<^sub>a \<Rightarrow> bool" 
   and fin_com\<^sub>a :: "'prog\<^sub>a"
+  and \<Gamma>\<^sub>a :: "'Env\<^sub>a"
   and C0\<^sub>a :: "('l\<^sub>a, 'k\<^sub>a, 's\<^sub>a, 'prog\<^sub>a) pesconf"
   and step\<^sub>a :: "('l\<^sub>a,'k\<^sub>a,'s\<^sub>a,'prog\<^sub>a, 'd) action \<Rightarrow> (('l\<^sub>a,'k\<^sub>a,'s\<^sub>a,'prog\<^sub>a) pesconf \<times> ('l\<^sub>a,'k\<^sub>a,'s\<^sub>a,'prog\<^sub>a) pesconf) set" 
   and interference\<^sub>a :: "'d \<Rightarrow> 'd \<Rightarrow> bool" 
